Parameterize auto diff algorithm by numerical values implementation.

theories/auto_diff.v
@@ -7,8 +7,39 @@ From iris.base_logic.lib Require Import iprop wsat invariants.
 From iris.program_logic  Require Import weakestpre.
 From hazel               Require Import notation weakestpre deep_handler.
 
+Unset Suggest Proof Using. 
 
-Section differentiation.
+
+Class DiffRing := {
+  R : Set;
+
+  rO   : R;
+  rI   : R;
+
+  radd  : R → R → R;
+  rmult : R → R → R;
+  req   : R → R → Prop;
+
+  DReq :> Equivalence req;
+  DRadd_ext  :> Proper (req ==> req ==> req) radd;
+  DRmult_ext :> Proper (req ==> req ==> req) rmult;
+
+  DRsemi_ring_theory : semi_ring_theory rO rI radd rmult req
+}.
+
+
+Declare Scope diff_ring_scope.
+Delimit Scope diff_ring_scope with dring.
+
+Notation "0" := rO : diff_ring_scope.
+Notation "1" := rI : diff_ring_scope.
+
+Infix "==" := req  (at level 70) : diff_ring_scope.
+
+Instance diff_ring_inhabited `{DiffRing} : Inhabited R := populate rO.
+
+
+Section mathematical_defs.
 
 Definition name := loc.
 
@@ -46,35 +77,35 @@ Definition emap {A B : Set} (f : A → B) : expr A → expr B :=
 Definition emap' {A B : Set} `{Countable A, Inhabited B} (E : gmap A B) : expr A → expr B :=
   emap (λ i, lookup_total i E).
 
-Definition eval_op : op → nat → nat → nat :=
-  λ op n n', match op with Add => n + n' | Mult => n * n' end%nat.
+Definition eval_op `{DiffRing} : op → R → R → R :=
+  λ op, match op with Add => radd | Mult => rmult end.
 
-Definition eval : expr nat → nat :=
-  fix eval (e : expr nat) {struct e} : nat :=
-    match e with ELeaf n => n | ENode op ea eb =>
+Definition eval `{DiffRing} : expr R → R :=
+  fix eval (e : expr R) {struct e} : R :=
+    match e with ELeaf r => r | ENode op ea eb =>
        eval_op op (eval ea) (eval eb)
     end.
 
-Definition diff_var {A : Set} `{EqDecision A} (r u : A) : nat :=
-  if (decide (r = u)) then 1%nat else 0%nat.
+Definition diff_var {A : Set} `{EqDecision A, DiffRing} (r u : A) : R :=
+  if (decide (r = u)) then 1%dring else 0%dring.
 
-Definition diff {A : Set} `{EqDecision A} (E : A → nat) : expr A → A → nat :=
-  fix diff (e : expr A) (u : A) {struct e} : nat :=
+Definition diff {A : Set} `{EqDecision A, DiffRing} (E : A → R) : expr A → A → R :=
+  fix diff (e : expr A) (u : A) {struct e} : R :=
     match e with
     | ELeaf r => diff_var r u
     | ENode Add ea eb =>
        let ad := diff ea u in
        let bd := diff eb u in
-       (ad + bd)%nat
+       (radd ad bd)
     | ENode Mult ea eb =>
        let av := eval (emap E ea) in
        let bv := eval (emap E eb) in
        let ad := diff ea u in
        let bd := diff eb u in
-       (ad * bv + av * bd)%nat
+       (radd (rmult ad bv) (rmult av bd))
     end.
 
-Definition diff' {A : Set} `{Countable A} (E : gmap A nat) : expr A → A → nat :=
+Definition diff' {A : Set} `{Countable A, DiffRing} (E : gmap A R) : expr A → A → R :=
   diff (λ i, lookup_total i E).
 
 Global Instance op_eq_dec : EqDecision op.
@@ -102,17 +133,6 @@ Proof.
   { intros Hvar. simpl. f_equal. apply Hvar. set_solver. }
 Qed.
 
-Lemma diff_ext {A : Set} `{EqDecision A} (f : A → nat) (g : A → nat) (e : expr A) (x : A) :
-  (∀ x, x ∈ variables e → f x = g x) →
-    diff f e x = diff g e x.
-Proof.
-  induction e as [[|] a IHa b IHb|]; [| |done].
-  { intros Hvar. rewrite //= IHa; [rewrite IHb; [done|]|]; set_solver. }
-  { intros Hvar. rewrite //= IHa; [rewrite IHb; [|]|]; [|set_solver|set_solver].
-    rewrite !(emap_ext f g); [done| |]; set_solver.
-  }
-Qed.
-
 Lemma interp_snoc K x op a b y :
   interp (K ++ [(x, (op, a, b))]) y =
     if (decide (x = y)) then
@@ -123,74 +143,6 @@ Proof. by rewrite /interp reverse_app. Qed.
 
 Lemma interp_nil y : interp [] y = ELeaf y.
 Proof. done. Qed.
-
-Lemma diff_var_eq {A : Set} `{EqDecision A} (r : A) : diff_var r r = 1%nat.
-Proof. by rewrite /diff_var decide_True. Qed.
-
-Lemma diff_var_neq {A : Set} `{EqDecision A} (r u : A) : r ≠ u → diff_var r u = 0%nat.
-Proof. intros ?. by rewrite /diff_var decide_False. Qed.
-
-Lemma eval_interp (E : gmap name nat) (K : let_expr) r x op a b av bv :
-  E !! a = Some av →
-  E !! b = Some bv →
-    eval (emap' E (interp ((x, (op, a, b)) :: K) r)) =
-      eval (emap' (<[x:=eval_op op av bv]> E) (interp K r)).
-Proof.
-  intros Heval_a Heval_b. rewrite -(reverse_involutive K).
-  revert r op; induction (reverse K) as [|(y, ((op', a'), b')) K']; intros r op.
-  { rewrite reverse_nil -(app_nil_l [(x, _)]) interp_snoc //=.
-    case (decide (x = r)).
-    { revert Heval_a Heval_b. simpl. rewrite !lookup_total_alt.
-      intros -> -> ->. by rewrite lookup_insert //=. }
-    { simpl. rewrite !lookup_total_alt.
-      intros ?. by rewrite lookup_insert_ne. }
-  }
-  { rewrite reverse_cons app_comm_cons !interp_snoc.
-    case (decide (y = r)); case op; case op'; try simpl; by rewrite !IHK'.
-  }
-Qed.
-
-Lemma diff_interp_cons av bv E K r u x op a b :
-  x ≠ u →
-  E !! a = Some av →
-  E !! b = Some bv →
-    diff' E (interp ((x, (op, a, b)) :: K) r) u =
-      let opd := diff' E (ENode op (ELeaf a) (ELeaf b)) u  in
-      let ud :=  diff' (<[x:=eval_op op av bv]> E) (interp K r) u in
-      let xd :=  diff' (<[x:=eval_op op av bv]> E) (interp K r) x in
-      (ud + opd * xd)%nat.
-Proof.
-  revert r u E. induction K as [|(y, ((op', a'), b')) K'] using rev_ind;
-  intros r u E Hneq Heval_a Heval_b.
-  { rewrite /interp //=. case (decide (x = r)).
-    { intros ->. by rewrite diff_var_eq (diff_var_neq _ _ Hneq) Nat.mul_1_r. }
-    { intros Hneq'. rewrite (diff_var_neq r x); [|done].
-      by rewrite Nat.mul_0_r Nat.add_0_r.
-    }
-  }
-  { rewrite app_comm_cons !interp_snoc //=.
-    case (decide (y = r)); case op'; try by rewrite !IHK'.
-    { intros ->. simpl. rewrite !IHK'; try done. simpl. lia. }
-    { intros ->. simpl.
-      rewrite !(eval_interp _ _ _ _ _ _ _ av bv); try done.
-      rewrite !IHK'; try done. simpl.  unfold emap'. lia.
-    }
-  }
-Qed.
-
-Lemma diff_emap (A B : Set) `{EqDecision A, EqDecision B} (f : A → B) (g : B → nat) (e : expr A) (x : A) :
-  (∀ y, y ∈ variables e → f x = f y → x = y) →
-      diff g (emap f e) (f x) = diff (g ∘ f) e x.
-Proof.
-  intros Hf_inj. induction e as [op ea IHea eb IHeb|y].
-  { simpl. rewrite !IHea; [rewrite !IHeb|]; [by rewrite emap_compose emap_compose| |];
-    intros ??; apply Hf_inj; rewrite elem_of_app; [by right|by left]. }
-  { case (decide (f y = f x)) as [Heq|Hneq]; simpl.
-    { specialize (Hf_inj y). rewrite Hf_inj; [by rewrite !diff_var_eq| |done].
-      by apply elem_of_list_singleton. }
-    { case (decide (y = x)) as [->|Hneq']; [done|]. by rewrite !diff_var_neq. }
-  }
-Qed.
 
 Lemma interp_app K K' x : x ∉ K'.*1 → interp (K ++ K') x = interp K x.
 Proof.
@@ -208,13 +160,144 @@ Proof.
   intros [Hnot_in [Hneq _]]. case (decide (y = x)); [by intros ->|]. by rewrite IHK'.
 Qed.
 
-End differentiation.
+Section diff_and_eval.
+
+  Context `{DiffRing}.
+
+  Add Ring DRing : DRsemi_ring_theory.
+
+  Lemma diff_ext {A : Set} `{EqDecision A} (f g : A → R) (e : expr A) (x : A) :
+    (∀ x, x ∈ variables e → f x = g x) →
+      diff f e x = diff g e x.
+  Proof.
+    induction e as [[|] a IHa b IHb|]; [| |done].
+    { intros Hvar. rewrite //= IHa; [rewrite IHb; [done|]|]; set_solver. }
+    { intros Hvar. rewrite //= IHa; [rewrite IHb; [|]|]; [|set_solver|set_solver].
+      rewrite !(emap_ext f g); [done| |]; set_solver.
+    }
+  Qed.
+
+  Lemma diff_var_eq {A : Set} `{EqDecision A} (r : A) :
+    diff_var r r = 1%dring.
+  Proof. by rewrite /diff_var decide_True. Qed.
+
+  Lemma diff_var_neq {A : Set } `{EqDecision A} (r u : A) :
+    r ≠ u → diff_var r u = 0%dring.
+  Proof. intros ?. by rewrite /diff_var decide_False. Qed.
+
+  Lemma eval_interp (E : gmap name R) (K : let_expr) r x op a b av bv :
+    E !! a = Some av →
+    E !! b = Some bv →
+      eval (emap' E (interp ((x, (op, a, b)) :: K) r)) =
+        eval (emap' (<[x:=eval_op op av bv]> E) (interp K r)).
+  Proof.
+    intros Heval_a Heval_b. rewrite -(reverse_involutive K).
+    revert r op; induction (reverse K) as [|(y, ((op', a'), b')) K']; intros r op.
+    { rewrite reverse_nil -(app_nil_l [(x, _)]) interp_snoc //=.
+      case (decide (x = r)).
+      { revert Heval_a Heval_b. simpl. rewrite !lookup_total_alt.
+        intros -> -> ->. by rewrite lookup_insert //=. }
+      { simpl. rewrite !lookup_total_alt.
+        intros ?. by rewrite lookup_insert_ne. }
+    }
+    { rewrite reverse_cons app_comm_cons !interp_snoc.
+      case (decide (y = r)); case op; case op'; try simpl; by rewrite !IHK'.
+    }
+  Qed.
+
+  Lemma diff_interp_cons av bv E K r u x op a b :
+    x ≠ u →
+    E !! a = Some av →
+    E !! b = Some bv →
+      req (diff' E (interp ((x, (op, a, b)) :: K) r) u)
+       (let opd := diff' E (ENode op (ELeaf a) (ELeaf b)) u  in
+        let ud :=  diff' (<[x:=eval_op op av bv]> E) (interp K r) u in
+        let xd :=  diff' (<[x:=eval_op op av bv]> E) (interp K r) x in
+        (radd ud (rmult opd xd))).
+  Proof.
+    revert r u E. induction K as [|(y, ((op', a'), b')) K'] using rev_ind;
+    intros r u E Hneq Heval_a Heval_b.
+    { rewrite /interp //=. case (decide (x = r)).
+      { intros ->. rewrite diff_var_eq (diff_var_neq _ _ Hneq).
+        destruct op; simpl; ring.
+      }
+      { intros Hneq'. rewrite (diff_var_neq r x); [|done].
+        destruct op; simpl; ring.
+      }
+    }
+    { rewrite app_comm_cons !interp_snoc //=.
+      case (decide (y = r)); case op'; try by rewrite !IHK'.
+      { intros ->. simpl. rewrite !IHK'; try done. destruct op; simpl; ring. }
+      { intros ->. simpl. rewrite !IHK'; try done. simpl.
+        rewrite !(eval_interp _ _ _ _ _ _ _ av bv); try done.
+        destruct op; simpl; unfold emap'; simpl; ring.
+      }
+    }
+  Qed.
+
+  Lemma diff_emap (A B : Set) `{EqDecision A, EqDecision B} (f : A → B) (g : B → R) (e : expr A) (x : A) :
+    (∀ y, y ∈ variables e → f x = f y → x = y) →
+        diff g (emap f e) (f x) = diff (g ∘ f) e x.
+  Proof.
+    intros Hf_inj. induction e as [op ea IHea eb IHeb|y].
+    { simpl. rewrite !IHea; [rewrite !IHeb|]; [by rewrite emap_compose emap_compose| |];
+      intros ??; apply Hf_inj; rewrite elem_of_app; [by right|by left]. }
+    { case (decide (f y = f x)) as [Heq|Hneq]; simpl.
+      { specialize (Hf_inj y). rewrite Hf_inj; [by rewrite !diff_var_eq| |done].
+        by apply elem_of_list_singleton. }
+      { case (decide (y = x)) as [->|Hneq']; [done|]. by rewrite !diff_var_neq. }
+    }
+  Qed.
+
+End diff_and_eval.
+
+End mathematical_defs.
 
 
 (** Implementation. *)
 
+Class Numeric `{!irisG eff_lang Σ, !DiffRing} := {
+
+  (* Language-level operations. *)
+
+  nO : val;
+  nI : val;
+
+  nadd  : val;
+  nmult : val;
+
+  repr : val → R → iProp Σ;
+
+  repr_pers a ra :> Persistent (repr a ra);
+  repr_ne a n : Proper (req ==> (dist n)) (repr a);
+
+  effs : iEff Σ;
+
+  nO_spec : ⊢ repr nO rO;
+  (* ⊢ EWP nO #() <| effs |> {{ c, repr c rO }}; *)
+
+  nI_spec : ⊢ repr nI rI;
+  (* ⊢ EWP nI #() <| effs |> {{ c, repr c rI }}; *)
+
+  nadd_spec (a b : val) (ra rb : R) :
+    repr a ra -∗
+      repr b rb -∗
+        EWP nadd a b <| effs |> {{ c, repr c (radd ra rb) }};
+
+  nmult_spec (a b : val) (ra rb : R) :
+    repr a ra -∗
+      repr b rb -∗
+        EWP nmult a b <| effs |> {{ c, repr c (rmult ra rb) }};
+
+}.
+
+Global Instance repr_proper `{!irisG eff_lang Σ, !DiffRing, !Numeric} a :
+  Proper (req ==> (≡)) (repr a).
+Proof. intros ???. apply equiv_dist=>n. by apply repr_ne. Qed.
+
+
 Section code.
-Context `{!heapG Σ}.
+Context `{!heapG Σ} `{!DiffRing} `{!Numeric}.
 
 Definition add : val := λ: "a" "b",
   do: InjL ("a", "b").
@@ -223,7 +306,7 @@ Definition mult : val := λ: "a" "b",
   do: InjR ("a", "b").
 
 Definition mk : val := λ: "x",
-  ref ("x", #0%nat).
+  ref ("x", nO).
 
 Definition get_val : val := λ: "x",
   Fst (Load "x").
@@ -242,24 +325,24 @@ Definition run : val := λ: "client",
         InjL "p" =>
           let: "a" := Fst "p" in
           let: "b" := Snd "p" in
-          let: "u" := mk ((get_val "a") + (get_val "b")) in
+          let: "u" := mk (nadd (get_val "a") (get_val "b")) in
           "k" "u";;
           let: "ud" := get_diff "u" in
-          set_diff "a" ((get_diff "a") + "ud");;
-          set_diff "b" ((get_diff "b") + "ud")
+          set_diff "a" (nadd (get_diff "a") "ud");;
+          set_diff "b" (nadd (get_diff "b") "ud")
       | InjR "p" =>
           let: "a" := Fst "p" in
           let: "b" := Snd "p" in
           let: "av" := get_val "a" in
           let: "bv" := get_val "b" in
-          let: "u" := mk ("av" * "bv") in
+          let: "u" := mk (nmult "av" "bv") in
           "k" "u";;
           let: "ud" := get_diff "u" in
-          set_diff "a" ((get_diff "a") + ("bv" * "ud"));;
-          set_diff "b" ((get_diff "b") + ("av" * "ud"))
+          set_diff "a" (nadd (get_diff "a") (nmult "bv" "ud"));;
+          set_diff "b" (nadd (get_diff "b") (nmult "av" "ud"))
       end)
   (* Return branch: *)
-  | return (λ: "r", set_diff "r" #1%nat)
+  | return (λ: "r", set_diff "r" nI)
   end.
 
 Definition grad : val := λ: "f" "n",
@@ -357,7 +440,7 @@ Proof. solve_inG. Qed.
 (** Ghost theory. *)
 
 Section ghost_theory_defs.
-Context `{!heapG Σ} `{!cgraphG Σ}.
+Context `{!heapG Σ, !cgraphG Σ, !DiffRing, !Numeric}.
 
 Definition to_cgraph : let_expr → gmap name node := list_to_map.
 
@@ -376,44 +459,47 @@ Definition represents γ (x : name) : name → expr unit → iProp Σ :=
         ⌜ x = y ⌝
     end%I.
 
-Definition handler_inv γ (x : name) (xv : nat) (K : let_expr) : iProp Σ :=
+Definition handler_inv γ (x : name) (xv : R) (K : let_expr) : iProp Σ :=
   (let_expr_auth γ K ∗
   ⌜ ∀ u, u ∈ K.*1 → variables (interp K u) ⊆ [x] ⌝ ∗
-  ([∗ list] u ∈ x :: K.*1,
-      u ↦ PairV #(eval (emap' {[x:=xv]} (interp K u))) #0%nat))%I.
+  ([∗ list] u ∈ x :: K.*1, ∃ uv,
+      repr uv (eval (emap' {[x:=xv]} (interp K u))) ∗
+      u ↦ PairV uv nO))%I.
 
-Definition env_extension (x : name) (xv : nat) (K : let_expr) : gmap name nat:=
+Definition env_extension (x : name) (xv : R) (K : let_expr) : gmap name R :=
   list_to_map ((λ '(u, _),
     (u, eval (emap' {[x:=xv]} (interp K u)))
   ) <$> K).
 
-Definition backpropagation_inv (x : name) (xv : nat) (K : let_expr) (e : expr unit) : iProp Σ :=
+Definition backpropagation_inv (x : name) (xv : R) (K : let_expr) (e : expr unit) : iProp Σ :=
   (∃ K' r,
      ⌜ interp (K ++ K') r = emap (λ _, x) e ⌝ ∗
   (* ⌜ ∀ u, u ∈ (x :: K.*1) → u ∈ K'.*1 → False ⌝ ∗ *)
   (* ⌜ ∀ u, u ∈ K.*1 → variables (interp K u) ⊆ [x] ⌝ ∗ *)
      let E := env_extension x xv K in
-     [∗ list] u ∈ x :: K.*1,
-        let uv := eval (emap' {[x:=xv]} (interp K u)) in
-        let ud := diff' (<[x:=xv]> E) (interp K' r) u in
-        u ↦ PairV #uv #ud)%I.
+     [∗ list] u ∈ x :: K.*1, ∃ uv ud,
+        repr uv (eval (emap' {[x:=xv]} (interp K u))) ∗
+        repr ud (diff' (<[x:=xv]> E) (interp K' r) u) ∗
+        u ↦ PairV uv ud)%I.
 
 End ghost_theory_defs.
 
 
 Section ghost_theory_proofs.
-Context `{!heapG Σ} `{!cgraphG Σ}.
+Context `{Hp: !heapG Σ, Cg: !cgraphG Σ, DR: !DiffRing, Num: !Numeric}.
 
 Global Instance represents_persistent γ x u uv : Persistent (represents γ x u uv).
 Proof. revert uv u. induction uv; intros ?; rewrite /ownI; apply _. Qed.
 
-Lemma handler_inv_alloc (x : name) (xv : nat) :
-  x ↦ (#xv, #0%nat) ==∗ ∃ γ, handler_inv γ x xv [].
+Lemma handler_inv_alloc (x : name) (uv : val) (xv : R) :
+  repr uv xv -∗
+    x ↦ (uv, nO) ==∗ ∃ γ, handler_inv γ x xv [].
 Proof.
-  iIntros "Hx". iMod (own_alloc (gmap_view_auth (V:=leibnizO node) 1 ∅))
+  iIntros "Hrepr Hx". iMod (own_alloc (gmap_view_auth (V:=leibnizO node) 1 ∅))
       as (γ) "Hauth". { apply gmap_view_auth_valid. }
   iModIntro. iExists γ. iFrame. rewrite //= lookup_total_singleton. iFrame.
-  iPureIntro; intros u. by rewrite elem_of_nil.
+  iSplit; [iPureIntro|iSplit; [iExists uv|]; by iFrame].
+  intros u. by rewrite elem_of_nil.
 Qed.
 
 Lemma cgraph_lookup γ (G : gmap name node) (x : name) (n : node) :
@@ -453,16 +539,16 @@ Qed.
 Lemma handler_inv_NoDup γ x xv K : handler_inv γ x xv K -∗ ⌜ NoDup (x :: K.*1) ⌝.
 Proof.
   iIntros "(_ & _ & HK)". iApply big_sepL_mapsto_NoDup.
-  iApply (big_sepL_mono with "HK"). iIntros (i u Hin) "Hu".
-  by iExists _.
+  iApply (big_sepL_mono with "HK"). iIntros (i u Hin). simpl.
+  iDestruct 1 as (uv) "[_ Hu]". by iExists _.
 Qed.
 
 Lemma backpropagation_inv_NoDup x xv K e :
   backpropagation_inv x xv K e -∗ ⌜ NoDup (x :: K.*1) ⌝.
 Proof.
   iDestruct 1 as (r K') "(_ & HK)". iApply big_sepL_mapsto_NoDup.
-  iApply (big_sepL_mono with "HK"). iIntros (i u Hin) "Hu".
-  by iExists _.
+  iApply (big_sepL_mono with "HK"). iIntros (i u Hin). simpl.
+  iDestruct 1 as (uv ud) "[_ [_ Hu]]". by iExists _.
 Qed.
 
 (* FIXME: move this lemma to a proper place (stdpp maybe?). *)
@@ -579,18 +665,19 @@ Proof.
   iIntros "Hu [_ [_ HK]]". iInduction (x :: K.*1) as [|y ys] "IH". 
   { iPureIntro. by apply not_elem_of_nil. }
   { rewrite not_elem_of_cons. simpl.
-    iDestruct "HK" as "[Hy HK]". iSplit.
+    iDestruct "HK" as "[Hy HK]". iDestruct "Hy" as (uv) "[_ Hy]". iSplit.
     { by iApply (mapsto_ne with "Hu Hy"). }
     { by iApply ("IH" with "Hu HK"). }
   }
 Qed.
 
-Lemma handler_inv_update γ x xv K u op a b av bv :
-  u ↦ PairV #(eval (emap' {[x:=xv]} (ENode op (interp K a) (interp K b)))) #0%nat -∗
-    handler_inv γ x xv K -∗ represents γ x a av -∗ represents γ x b bv ==∗
-      handler_inv γ x xv (K ++ [(u, (op, a, b))]) ∗ represents γ x u (ENode op av bv).
+Lemma handler_inv_update γ x xv K u op a b av bv uv :
+  repr uv (eval (emap' {[x:=xv]} (ENode op (interp K a) (interp K b)))) -∗
+    u ↦ PairV uv nO -∗
+      handler_inv γ x xv K -∗ represents γ x a av -∗ represents γ x b bv ==∗
+        handler_inv γ x xv (K ++ [(u, (op, a, b))]) ∗ represents γ x u (ENode op av bv).
 Proof.
-  iIntros "Hu Hhandler_inv Ha Hb".
+  iIntros "Huv Hu Hhandler_inv Ha Hb".
   iDestruct (handler_inv_elem_of' with "Hhandler_inv Ha") as %Ha_in%elem_of_cons.
   iDestruct (handler_inv_elem_of' with "Hhandler_inv Hb") as %Hb_in%elem_of_cons.
   iDestruct (handler_inv_fresh_name with "Hu Hhandler_inv")
@@ -613,7 +700,8 @@ Proof.
     case Hb_in as [->|Hb_in]; [rewrite Hx| |rewrite Hx|]; set_solver.
   }
   { rewrite fmap_app fmap_cons fmap_nil app_comm_cons big_sepL_app.
-    iSplitL "HK"; [|by rewrite //= interp_snoc decide_True; [iFrame|]].
+    iSplitL "HK"; [|
+    by rewrite //= interp_snoc decide_True; [iSplit; [iExists uv; iFrame|]|]].
     have H: u ∉ x :: K.*1; [set_solver|]. clear Hvar HNoDup Hneq Hnot_in.
     iRevert (H). iInduction (x :: K.*1) as [|y ys] "IH"; [by iIntros (?)|].
     rewrite not_elem_of_cons. iIntros ([Hneq H]). iDestruct "HK" as "[Hy HK]".
@@ -671,26 +759,19 @@ Proof.
   { by rewrite lookup_insert_ne; [apply lookup_env_extension|intros ->]. }
 Qed.
 
-(*Lemma handler_inv_backpropagation_inv E e γ x xv K r rv :
-  (r ↦ PairV #(eval (emap' {[x:=xv]} (emap (λ _, x) rv))) #0%nat -∗
-    EWP e @ E {{_, r ↦ PairV #(eval (emap' {[x:=xv]} (emap (λ _, x) rv))) #1%nat }}) -∗
-      handler_inv γ x xv K -∗ represents γ x r rv -∗
-        EWP e @ E {{ _, backpropagation_inv x xv K rv }}.
-Proof.
-  iIntros "He Hhinv Hr".
-Qed.*)
-
 End ghost_theory_proofs.
 
 
 (** Verification. *)
 
 Section verification.
-Context `{!heapG Σ} `{!cgraphG Σ}.
+Context `{Hp: !heapG Σ, Cg: !cgraphG Σ, DR: !DiffRing, Num: !Numeric}.
 
-Lemma set_diff_spec E x xv xd xd' :
-  x ↦ PairV #xv #xd -∗
-    EWP set_diff #x #xd' @ E {{ _, x ↦ PairV #xv #xd' }}.
+Add Ring DRing : DRsemi_ring_theory.
+
+Lemma set_diff_spec E Ψ (x : name) (xv xd xd' : val) :
+  x ↦ PairV xv xd -∗
+    EWP set_diff #x xd' @ E <| Ψ |> {{ _, x ↦ PairV xv xd' }}.
 Proof.
   iIntros "Hx". iApply (Ectxi_ewp_bind (AppLCtx _)). done.
   iApply ewp_pure_step. apply pure_prim_step_beta. simpl.
@@ -706,9 +787,9 @@ Proof.
   by iApply (ewp_store with "Hx").
 Qed.
 
-Lemma get_diff_spec E x xv xd :
-  x ↦ PairV #xv #xd -∗
-    EWP get_diff #x @ E {{ y, ⌜ y = #xd ⌝ ∗ x ↦ PairV #xv #xd }}.
+Lemma get_diff_spec E Ψ (x : name) (xv xd : val) :
+  x ↦ PairV xv xd -∗
+    EWP get_diff #x @ E <| Ψ |> {{ y, ⌜ y = xd ⌝ ∗ x ↦ PairV xv xd }}.
   iIntros "Hx".
   iApply ewp_pure_step. apply pure_prim_step_beta. simpl.
   iApply (Ectxi_ewp_bind SndCtx). done.
@@ -718,11 +799,11 @@ Lemma get_diff_spec E x xv xd :
   by iFrame.
 Qed.
 
-Lemma get_val_spec γ x xv K u uv :
+Lemma get_val_spec E Ψ γ x xv K u uv :
   represents γ x u uv -∗
     handler_inv γ x xv K -∗
-      EWP get_val #u {{ y,
-        ⌜ y = #(eval (emap' {[x:=xv]} (emap (λ _, x) uv))) ⌝ ∗
+      EWP get_val #u @ E <| Ψ |> {{ y,
+        repr y (eval (emap' {[x:=xv]} (emap (λ _, x) uv))) ∗
           handler_inv γ x xv K }}.
 Proof.
   iIntros "Hu Hhinv".
@@ -735,17 +816,18 @@ Proof.
   iDestruct "HK" as "[Hu' HK]".
   iApply ewp_pure_step. apply pure_prim_step_beta. simpl.
   iApply (Ectxi_ewp_bind FstCtx). done.
+  iDestruct "Hu'" as (uv') "[#Hrepr Hu']".
   iApply (ewp_mono' with "[Hu']"). { by iApply (ewp_load with "Hu'"). }
   iIntros (y) "[-> Hu']". iModIntro. simpl.
   iApply ewp_pure_step. apply pure_prim_step_Fst. iApply ewp_value.
-  rewrite -!Hinterp. iSplit; [done|]. iFrame.
+  rewrite -!Hinterp. iFrame. iSplit; [done|]. iFrame.
   rewrite HK_eq. rewrite (big_opL_permutation _ (us ++ _) (u :: (vs ++ us))); [|
   by rewrite Permutation_app_comm].
-  by iFrame.
+  iFrame. iExists uv'. by iFrame.
 Qed.
 
-Lemma mk_spec E (xv : val) :
-  ⊢ EWP mk xv @ E {{ y, ∃ (x : name), ⌜ y = #x ⌝ ∗ x ↦ (PairV xv #0%nat) }}.
+Lemma mk_spec E Ψ (xv : val) :
+  ⊢ EWP mk xv @ E <| Ψ |> {{ y, ∃ (x : name), ⌜ y = #x ⌝ ∗ x ↦ (PairV xv nO) }}.
 Proof.
   iApply ewp_pure_step. apply pure_prim_step_beta. simpl.
   iApply (Ectxi_ewp_bind AllocCtx). done.
@@ -753,9 +835,9 @@ Proof.
   by iApply ewp_alloc.
 Qed.
 
-Lemma return_spec γ x xv K r (e : expr unit) :
+Lemma return_spec E Ψ γ x xv K r (e : expr unit) :
   handler_inv γ x xv K -∗ represents γ x r e -∗ 
-    EWP set_diff #r #1%nat {{ _, backpropagation_inv x xv K e }}.
+    EWP set_diff #r nI @ E <| Ψ |> {{ _, backpropagation_inv x xv K e }}.
 Proof.
   iIntros "Hhinv Hrepr".
   iDestruct (handler_inv_agree with "Hhinv Hrepr") as %Hinterp.
@@ -763,24 +845,27 @@ Proof.
   iDestruct (handler_inv_NoDup with "Hhinv") as %HNoDup.
   iDestruct "Hhinv" as "[_ [Hvar HK]]". iClear "Hrepr".
   iDestruct (big_sepL_delete' _ _ _ _ Hin with "HK") as "[Hu HK]".
-  iApply (ewp_mono' with "[Hu]"). { by iApply (set_diff_spec with "Hu"). }
-  iIntros (_) "Hu !>". iExists [], r. rewrite app_nil_r Hinterp.
-  (* iSplit; [done|]. iSplit; [iIntros (?); by rewrite elem_of_nil|]. *) iSplit; [done|].
-  rewrite (big_sepL_delete' (λ _ u, u ↦ (_, #(diff' _ _ _)))%I _ _ _ Hin).
-  iSplitL "Hu"; [by rewrite //= Hinterp diff_var_eq|].
-  iApply (big_sepL_mono with "HK").
-  iIntros (k v Hin') "Hv". iIntros (Hneq). iSpecialize ("Hv" $! Hneq).
-  rewrite //= diff_var_neq; [done|]. intros ->.
-  by destruct (NoDup_lookup _ _ _ _ HNoDup Hin Hin').
+  iDestruct "Hu" as (uv) "[Huv Hr]".
+  iApply (ewp_mono' with "[Hr]"). { by iApply (set_diff_spec with "Hr"). }
+  iIntros (_) "Hr !>". iExists [], r. rewrite app_nil_r Hinterp.
+  iSplit; [done|].
+  rewrite (big_sepL_delete' (λ _ u, ∃ uv ud, _ ∗ _ ∗ _)%I _ _ _ Hin).
+  iSplitL "Huv Hr".
+  - iExists uv, nI. rewrite //= Hinterp diff_var_eq. iFrame. iApply nI_spec.
+  - iApply (big_sepL_mono with "HK").
+    iIntros (k v Hin') "Hv". iIntros (Hneq).
+    iDestruct ("Hv" $! Hneq) as (vv) "[Hvv Hv]". iExists vv, nO. iFrame.
+    rewrite //= diff_var_neq; [iApply nO_spec|]. intros ->.
+    by destruct (NoDup_lookup _ _ _ _ HNoDup Hin Hin').
 Qed.
 
 Lemma add_update_spec_1 x xv K u a e :
   NoDup (x :: K.*1) → a ∈ x :: K.*1 → u ∉ x :: K.*1 →
     backpropagation_inv x xv (K ++ [(u, (Add, a, a))]) e -∗
       EWP let: "ud" := get_diff #u in
-          set_diff #a ((get_diff #a) + "ud");;
-          set_diff #a ((get_diff #a) + "ud")
-      {{_, backpropagation_inv x xv K e }}.
+          set_diff #a (nadd (get_diff #a) "ud");;
+          set_diff #a (nadd (get_diff #a) "ud")
+      <| effs |> {{_, backpropagation_inv x xv K e }}.
 Proof.
   intros HNoDup Hin Hnot_in.
   iDestruct 1 as (K' r) "(% & HK)". rename H into Hr.
@@ -788,6 +873,8 @@ Proof.
   assert (∃ l, l = (x :: K.*1)) as [l Hl]; [by eauto|].
   destruct (elem_of_list_lookup_1 _ _ Hin) as [i Hlkp].
   iDestruct (big_sepL_delete' _ _ _ _ Hlkp with "HK") as "[Ha HK]".
+  iDestruct "Hu" as (uv ud) "(#Hrepr_uv & #Hrepr_ud & Hu)".
+  iDestruct "Ha" as (av ad) "(#Hrepr_av & #Hrepr_ad & Ha)".
   iApply (Ectxi_ewp_bind (AppRCtx _)). done. rewrite -Hl //=.
   iApply (ewp_mono' with "[Hu]"). { by iApply (get_diff_spec with "Hu"). }
   iIntros (v) "[-> Hu]". iModIntro.
@@ -796,20 +883,24 @@ Proof.
   iApply ewp_pure_step. apply pure_prim_step_beta. simpl.
   iApply (Ectxi_ewp_bind (AppRCtx _)). done.
   iApply (Ectxi_ewp_bind (AppRCtx _)). done.
-  iApply (Ectxi_ewp_bind (BinOpLCtx _ _)). done.
+  iApply (ewp_bind (ConsCtx (AppLCtx _)
+                   (ConsCtx (AppRCtx _) EmptyCtx))). done.
   iApply (ewp_mono' with "[Ha]"). { by iApply (get_diff_spec with "Ha"). }
   iIntros (y) "[-> Ha]". iModIntro. simpl.
-  iApply ewp_pure_step. by apply pure_prim_step_binop. iApply ewp_value.
+  iApply ewp_mono'. { by iApply (nadd_spec with "Hrepr_ad Hrepr_ud"). }
+  iIntros (ad') "#Hrepr_ad'". iModIntro. iClear "Hrepr_ad".
   iApply (ewp_mono' with "[Ha]"). { by iApply (set_diff_spec with "Ha"). }
   iIntros (v) "Ha". iModIntro.
   iApply (Ectxi_ewp_bind (AppLCtx _)). done.
   iApply ewp_pure_step. apply pure_prim_step_rec. iApply ewp_value. simpl.
   iApply ewp_pure_step. apply pure_prim_step_beta. simpl.
   iApply (Ectxi_ewp_bind (AppRCtx _)). done.
-  iApply (Ectxi_ewp_bind (BinOpLCtx _ _)). done.
+  iApply (ewp_bind (ConsCtx (AppLCtx _)
+                   (ConsCtx (AppRCtx _) EmptyCtx))). done.
   iApply (ewp_mono' with "[Ha]"). { by iApply (get_diff_spec with "Ha"). }
   iIntros (y) "[-> Ha]". iModIntro. simpl.
-  iApply ewp_pure_step. by apply pure_prim_step_binop. iApply ewp_value.
+  iApply ewp_mono'. { by iApply (nadd_spec with "Hrepr_ad' Hrepr_ud"). }
+  iIntros (ad'') "#Hrepr_ad''". iModIntro. iClear "Hrepr_ad'".
   iApply (ewp_mono' with "[Ha]"). { by iApply (set_diff_spec with "Ha"). }
   clear v. iIntros (v) "Ha". iModIntro.
   iExists ((u, (Add, a, a)) :: K'), r.
@@ -817,23 +908,31 @@ Proof.
   rewrite (big_sepL_delete' _ _ _ _ Hlkp).
   have Hneq: a ≠ u. { by intros ->. }
   iClear "Hu". iSplitL "Ha"; [|rewrite Hl; iApply (big_sepL_mono with "HK")].
-  { rewrite interp_snoc decide_False; [|done].
+  { iExists av, ad''. iFrame. iClear "Hrepr_uv Hrepr_ud".
+    iSplit; [by rewrite interp_snoc decide_False|]. iClear "Hrepr_av".
+    iApply (repr_proper with "Hrepr_ad''").
     rewrite (diff_interp_cons (eval (emap' {[x:=xv]} (interp K a)))
                               (eval (emap' {[x:=xv]} (interp K a))));
     try (by apply lookup_env_extension'); try done.
     rewrite -env_extension_app'; [|done]. simpl. rewrite diff_var_eq //=.
-    rewrite Nat.add_0_r Nat.add_assoc !Nat2Z.inj_add. done.
+    rewrite (_ : ∀ x y,
+      radd x (rmult (radd 1 1) y) == radd (radd x y) y)%dring; [done|].
+    intros ??. ring.
   }
   { intros k y Hlkp'. simpl. iIntros "Hy". iIntros (Hneq').
     have Hneq'': u ≠ y; [
     intros ->; by apply Hnot_in, (elem_of_list_lookup_2 _ k)|].
-    iSpecialize ("Hy" $! Hneq'). rewrite interp_snoc decide_False; [|done].
+    iDestruct ("Hy" $! Hneq') as (yv yd) "(Hrepr_yv & Hrepr_yd & Hy)".
+    iExists yv, yd. iFrame.
+    rewrite interp_snoc decide_False; [|done]. iFrame.
+    iApply (repr_proper with "Hrepr_yd").
     rewrite (diff_interp_cons (eval (emap' {[x:=xv]} (interp K a)))
                               (eval (emap' {[x:=xv]} (interp K a))));
     try (by apply lookup_env_extension'); try done.
     rewrite -env_extension_app'; [|done]. simpl. rewrite diff_var_neq //=;[|
     by intros ->; destruct (NoDup_lookup _ _ _ _ HNoDup Hlkp Hlkp')].
-    rewrite Nat.add_0_r. done.
+    rewrite (_ : ∀ x y, radd x (rmult (radd 0 0) y) == x)%dring; [done|].
+    intros ??. ring.
   }
 Qed.
 
@@ -841,9 +940,9 @@ Lemma add_update_spec_2 x xv K u a b e :
   NoDup (x :: K.*1) → a ∈ x :: K.*1 → b ∈ x :: K.*1 → a ≠ b → u ∉ x :: K.*1 →
     backpropagation_inv x xv (K ++ [(u, (Add, a, b))]) e -∗
       EWP let: "ud" := get_diff #u in
-          set_diff #a ((get_diff #a) + "ud");;
-          set_diff #b ((get_diff #b) + "ud")
-      {{_, backpropagation_inv x xv K e }}.
+          set_diff #a (nadd (get_diff #a) "ud");;
+          set_diff #b (nadd (get_diff #b) "ud")
+      <| effs |> {{_, backpropagation_inv x xv K e }}.
 Proof.
   intros HNoDup Ha_in Hb_in Hab Hnot_in.
   iDestruct 1 as (K' r) "(% & HK)". rename H into Hr.
@@ -856,6 +955,9 @@ Proof.
   have Hij: i ≠ j; [
   by intros ->; cut (Some a = Some b); [inversion 1|rewrite -Hlkp_a -Hlkp_b]|].
   iSpecialize ("Hb" with "[]"); [done|].
+  iDestruct "Hu" as (uv ud) "(#Hrepr_uv & #Hrepr_ud & Hu)".
+  iDestruct "Ha" as (av ad) "(#Hrepr_av & #Hrepr_ad & Ha)".
+  iDestruct "Hb" as (bv bd) "(#Hrepr_bv & #Hrepr_bd & Hb)".
   iApply (Ectxi_ewp_bind (AppRCtx _)). done. rewrite -Hl //=.
   iApply (ewp_mono' with "[Hu]"). { by iApply (get_diff_spec with "Hu"). }
   iIntros (v) "[-> Hu]". iModIntro.
@@ -864,20 +966,24 @@ Proof.
   iApply ewp_pure_step. apply pure_prim_step_beta. simpl.
   iApply (Ectxi_ewp_bind (AppRCtx _)). done.
   iApply (Ectxi_ewp_bind (AppRCtx _)). done.
-  iApply (Ectxi_ewp_bind (BinOpLCtx _ _)). done.
+  iApply (ewp_bind (ConsCtx (AppLCtx _)
+                   (ConsCtx (AppRCtx _) EmptyCtx))). done.
   iApply (ewp_mono' with "[Ha]"). { by iApply (get_diff_spec with "Ha"). }
   iIntros (y) "[-> Ha]". iModIntro. simpl.
-  iApply ewp_pure_step. by apply pure_prim_step_binop. iApply ewp_value.
+  iApply ewp_mono'. { by iApply (nadd_spec with "Hrepr_ad Hrepr_ud"). }
+  iIntros (ad') "#Hrepr_ad'". iModIntro. iClear "Hrepr_ad".
   iApply (ewp_mono' with "[Ha]"). { by iApply (set_diff_spec with "Ha"). }
   iIntros (v) "Ha". iModIntro.
   iApply (Ectxi_ewp_bind (AppLCtx _)). done.
   iApply ewp_pure_step. apply pure_prim_step_rec. iApply ewp_value. simpl.
   iApply ewp_pure_step. apply pure_prim_step_beta. simpl.
   iApply (Ectxi_ewp_bind (AppRCtx _)). done.
-  iApply (Ectxi_ewp_bind (BinOpLCtx _ _)). done.
+  iApply (ewp_bind (ConsCtx (AppLCtx _)
+                   (ConsCtx (AppRCtx _) EmptyCtx))). done.
   iApply (ewp_mono' with "[Hb]"). { by iApply (get_diff_spec with "Hb"). }
   iIntros (y) "[-> Hb]". iModIntro. simpl.
-  iApply ewp_pure_step. by apply pure_prim_step_binop. iApply ewp_value.
+  iApply ewp_mono'. { by iApply (nadd_spec with "Hrepr_bd Hrepr_ud"). }
+  iIntros (bd') "#Hrepr_bd'". iModIntro. iClear "Hrepr_bd".
   iApply (ewp_mono' with "[Hb]"). { by iApply (set_diff_spec with "Hb"). }
   clear v. iIntros (v) "Hb". iModIntro.
   iExists ((u, (Add, a, b)) :: K'), r.
@@ -886,23 +992,32 @@ Proof.
   rewrite (big_sepL_delete' _ _ _ _ Hlkp_b).
   have Hau: a ≠ u. { by intros ->. }
   have Hbu: b ≠ u. { by intros ->. }
-  iClear "Hu". rewrite !interp_snoc !decide_False; try done.
-  rewrite !(diff_interp_cons (eval (emap' {[x:=xv]} (interp K a)))
-                             (eval (emap' {[x:=xv]} (interp K b))));
-    try (by apply lookup_env_extension'); try done.
-  rewrite -!env_extension_app'; [|done].
+  iClear "Hu". rewrite interp_snoc decide_True;[|done].
+  rewrite !interp_snoc !decide_False; try done.
   iSplitL "Ha"; [|iSplitL "Hb"; [|rewrite Hl; iApply (big_sepL_mono with "HK")]].
-  { by simpl; rewrite diff_var_eq diff_var_neq; [
-    rewrite Nat.add_0_r Nat.add_assoc Nat.add_0_r !Nat2Z.inj_add|].
+  { iExists av, ad'. iFrame. iSplit; [iApply "Hrepr_av"|].
+    iApply (repr_proper with "Hrepr_ad'").
+    rewrite !(diff_interp_cons (eval (emap' {[x:=xv]} (interp K a)))
+                               (eval (emap' {[x:=xv]} (interp K b))));
+    try (by apply lookup_env_extension'); try done. simpl.
+    rewrite diff_var_eq diff_var_neq; [|done].
+    rewrite env_extension_app'; [|done]; simpl. ring.
   }
-  { iIntros (_). by simpl; rewrite diff_var_eq diff_var_neq; [
-    rewrite Nat.add_0_l Nat.add_assoc Nat.add_0_r !Nat2Z.inj_add|].
+  { iIntros (_). iExists bv, bd'. iFrame. iSplit; [iApply "Hrepr_bv"|].
+    iApply (repr_proper with "Hrepr_bd'").
+    rewrite !(diff_interp_cons (eval (emap' {[x:=xv]} (interp K a)))
+                               (eval (emap' {[x:=xv]} (interp K b))));
+    try (by apply lookup_env_extension'); try done. simpl.
+    rewrite diff_var_eq diff_var_neq; [|done].
+    rewrite env_extension_app'; [|done]; simpl. ring.
   }
   { intros k y Hlkp'. simpl. iIntros "Hy". iIntros (Hkj Hki).
-    iSpecialize ("Hy" $! Hkj Hki).
+    iDestruct ("Hy" $! Hkj Hki) as (yv yd) "(Hyv & Hyd & Hy)".
+    iExists yv, yd.
     have Hneq'': u ≠ y; [
     intros ->; by apply Hnot_in, (elem_of_list_lookup_2 _ k)|].
-    rewrite interp_snoc decide_False; [|done].
+    rewrite interp_snoc decide_False; [|done]. iFrame.
+    iApply (repr_proper with "Hyd").
     rewrite (diff_interp_cons (eval (emap' {[x:=xv]} (interp K a)))
                               (eval (emap' {[x:=xv]} (interp K b))));
     try (by apply lookup_env_extension'); try done.
@@ -911,25 +1026,29 @@ Proof.
     by intros ->; destruct (NoDup_lookup _ _ _ _ HNoDup Hlkp_a Hlkp')].
     rewrite diff_var_neq //=;[|
     by intros ->; destruct (NoDup_lookup _ _ _ _ HNoDup Hlkp_b Hlkp')].
-    rewrite Nat.add_0_r. done. 
+    rewrite (_ : ∀ x y, radd x (rmult (radd 0 0) y) == x)%dring; [done|].
+    intros ??. ring.
   }
 Qed.
 
-Lemma mult_update_spec_1 x xv K u a e :
-  let av := eval (emap' {[x:=xv]} (interp K a)) in
+Lemma mult_update_spec_1 x xv K u a e e_av e_bv :
   NoDup (x :: K.*1) → a ∈ x :: K.*1 → u ∉ x :: K.*1 →
+  repr e_av (eval (emap' {[x:=xv]} (interp K a))) -∗
+  repr e_bv (eval (emap' {[x:=xv]} (interp K a))) -∗
     backpropagation_inv x xv (K ++ [(u, (Mult, a, a))]) e -∗
       EWP let: "ud" := get_diff #u in
-          set_diff #a ((get_diff #a) + (#av * "ud"));;
-          set_diff #a ((get_diff #a) + (#av * "ud"))
-      {{_, backpropagation_inv x xv K e }}.
+          set_diff #a (nadd (get_diff #a) (nmult e_bv "ud"));;
+          set_diff #a (nadd (get_diff #a) (nmult e_av "ud"))
+      <| effs |> {{_, backpropagation_inv x xv K e }}.
 Proof.
-  simpl. intros HNoDup Hin Hnot_in.
+  simpl. intros HNoDup Hin Hnot_in. iIntros "#Heval_a #Heval_b".
   iDestruct 1 as (K' r) "(% & HK)". rename H into Hr.
   rewrite fmap_app fmap_cons app_comm_cons big_opL_app. iDestruct "HK" as "[HK [Hu _]]".
   assert (∃ l, l = (x :: K.*1)) as [l Hl]; [by eauto|].
   destruct (elem_of_list_lookup_1 _ _ Hin) as [i Hlkp].
   iDestruct (big_sepL_delete' _ _ _ _ Hlkp with "HK") as "[Ha HK]".
+  iDestruct "Hu" as (uv ud) "(#Hrepr_uv & #Hrepr_ud & Hu)".
+  iDestruct "Ha" as (av ad) "(#Hrepr_av & #Hrepr_ad & Ha)".
   iApply (Ectxi_ewp_bind (AppRCtx _)). done. rewrite -Hl //=.
   iApply (ewp_mono' with "[Hu]"). { by iApply (get_diff_spec with "Hu"). }
   iIntros (v) "[-> Hu]". iModIntro.
@@ -938,65 +1057,75 @@ Proof.
   iApply ewp_pure_step. apply pure_prim_step_beta. simpl.
   iApply (Ectxi_ewp_bind (AppRCtx _)). done.
   iApply (Ectxi_ewp_bind (AppRCtx _)). done.
-  iApply (Ectxi_ewp_bind (BinOpRCtx _ _)). done.
-  iApply ewp_pure_step. by apply pure_prim_step_binop. iApply ewp_value. simpl.
-  iApply (Ectxi_ewp_bind (BinOpLCtx _ _)). done.
+  iApply (Ectxi_ewp_bind (AppRCtx _)). done.
+  iApply ewp_mono'. { by iApply (nmult_spec with "Heval_b Hrepr_ud"). }
+  iIntros (c) "#Hc". iModIntro. simpl.
+  iApply (ewp_bind (ConsCtx (AppLCtx _)
+                   (ConsCtx (AppRCtx _) EmptyCtx))). done.
   iApply (ewp_mono' with "[Ha]"). { by iApply (get_diff_spec with "Ha"). }
   iIntros (y) "[-> Ha]". iModIntro. simpl.
-  iApply ewp_pure_step. by apply pure_prim_step_binop. iApply ewp_value.
+  iApply ewp_mono'. { by iApply (nadd_spec with "Hrepr_ad Hc"). }
+  iIntros (ad') "#Hrepr_ad'". iModIntro.
   iApply (ewp_mono' with "[Ha]"). { by iApply (set_diff_spec with "Ha"). }
-  iIntros (v) "Ha". iModIntro.
+  iIntros (v) "Ha". iModIntro. iClear "Hrepr_ad Hc". clear c ad.
   iApply (Ectxi_ewp_bind (AppLCtx _)). done.
   iApply ewp_pure_step. apply pure_prim_step_rec. iApply ewp_value. simpl.
   iApply ewp_pure_step. apply pure_prim_step_beta. simpl.
   iApply (Ectxi_ewp_bind (AppRCtx _)). done.
-  iApply (Ectxi_ewp_bind (BinOpRCtx _ _)). done.
-  iApply ewp_pure_step. by apply pure_prim_step_binop. iApply ewp_value. simpl.
-  iApply (Ectxi_ewp_bind (BinOpLCtx _ _)). done.
+  iApply (Ectxi_ewp_bind (AppRCtx _)). done.
+  iApply ewp_mono'. { by iApply (nmult_spec with "Heval_a Hrepr_ud"). }
+  iIntros (c) "#Hc". iModIntro. simpl.
+  iApply (ewp_bind (ConsCtx (AppLCtx _)
+                   (ConsCtx (AppRCtx _) EmptyCtx))). done.
   iApply (ewp_mono' with "[Ha]"). { by iApply (get_diff_spec with "Ha"). }
   iIntros (y) "[-> Ha]". iModIntro. simpl.
-  iApply ewp_pure_step. by apply pure_prim_step_binop. iApply ewp_value.
+  iApply ewp_mono'. { by iApply (nadd_spec with "Hrepr_ad' Hc"). }
+  iIntros (ad'') "#Hrepr_ad''". iModIntro.
   iApply (ewp_mono' with "[Ha]"). { by iApply (set_diff_spec with "Ha"). }
-  clear v. iIntros (v) "Ha". iModIntro.
+  clear v. iIntros (v) "Ha". iModIntro. iClear "Hrepr_ad' Hc". clear c v ad'.
   iExists ((u, (Mult, a, a)) :: K'), r.
   iSplit; [iPureIntro; by rewrite cons_middle app_assoc Hr|].
   rewrite (big_sepL_delete' _ _ _ _ Hlkp).
   have Hau: a ≠ u. { by intros ->. }
-  iClear "Hu". rewrite !interp_snoc !decide_False; try done.
-  rewrite !(diff_interp_cons (eval (emap' {[x:=xv]} (interp K a)))
-                             (eval (emap' {[x:=xv]} (interp K a))));
-    try (by apply lookup_env_extension'); try done.
-  rewrite -!env_extension_app'; [|done].
+  iClear "Hu Hrepr_uv Hrepr_ud Heval_a".
+  rewrite interp_snoc decide_False; try done.
   iSplitL "Ha"; [|rewrite Hl; iApply (big_sepL_mono with "HK")].
-  { rewrite //= diff_var_eq lookup_total_alt lookup_env_extension' //=.
-    rewrite Nat.mul_1_r Nat.add_0_r Nat.mul_add_distr_r Nat.add_assoc.
-    rewrite !Nat2Z.inj_add Nat2Z.inj_mul. done.
+  { iExists av, ad''. iFrame. iSplit; [done|].
+    iApply (repr_proper with "Hrepr_ad''").
+    rewrite !(diff_interp_cons (eval (emap' {[x:=xv]} (interp K a)))
+                               (eval (emap' {[x:=xv]} (interp K a))));
+    try (by apply lookup_env_extension'); try done.
+    rewrite -!env_extension_app'; [|done].
+    rewrite //= diff_var_eq lookup_total_alt lookup_env_extension' //=. ring.
   }
   { intros k y Hlkp'. simpl. iIntros "Hy". iIntros (Hki).
-    iSpecialize ("Hy" $! Hki). have Hneq'': u ≠ y; [
+    iDestruct ("Hy" $! Hki) as (yv yd) "(Hyv & Hyd & Hy)".
+    iExists yv, yd. iFrame.
+    have Hneq'': u ≠ y; [
     intros ->; by apply Hnot_in, (elem_of_list_lookup_2 _ k)|].
-    rewrite interp_snoc decide_False; [|done].
+    rewrite interp_snoc decide_False; [|done]. iFrame.
+    iApply (repr_proper with "Hyd").
     rewrite (diff_interp_cons (eval (emap' {[x:=xv]} (interp K a)))
                               (eval (emap' {[x:=xv]} (interp K a))));
     try (by apply lookup_env_extension'); try done.
     rewrite -env_extension_app'; [|done]. simpl.
     rewrite diff_var_neq //=;[|
     by intros ->; destruct (NoDup_lookup _ _ _ _ HNoDup Hlkp Hlkp')].
-    rewrite Nat.mul_0_r Nat.mul_0_l Nat.add_0_r. done. 
+    ring.
   }
 Qed.
 
-Lemma mult_update_spec_2 x xv K u a b e :
-  let av := eval (emap' {[x:=xv]} (interp K a)) in
-  let bv := eval (emap' {[x:=xv]} (interp K b)) in
+Lemma mult_update_spec_2 x xv K u a b e e_av e_bv :
   NoDup (x :: K.*1) → a ∈ x :: K.*1 → b ∈ x :: K.*1 → a ≠ b → u ∉ x :: K.*1 →
+  repr e_av (eval (emap' {[x:=xv]} (interp K a))) -∗
+  repr e_bv (eval (emap' {[x:=xv]} (interp K b))) -∗
     backpropagation_inv x xv (K ++ [(u, (Mult, a, b))]) e -∗
       EWP let: "ud" := get_diff #u in
-          set_diff #a ((get_diff #a) + (#bv * "ud"));;
-          set_diff #b ((get_diff #b) + (#av * "ud"))
-      {{_, backpropagation_inv x xv K e }}.
+          set_diff #a (nadd (get_diff #a) (nmult e_bv "ud"));;
+          set_diff #b (nadd (get_diff #b) (nmult e_av "ud"))
+      <| effs |> {{_, backpropagation_inv x xv K e }}.
 Proof.
-  simpl. intros HNoDup Ha_in Hb_in Hab Hnot_in.
+  simpl. intros HNoDup Ha_in Hb_in Hab Hnot_in. iIntros "#Heval_a #Heval_b".
   iDestruct 1 as (K' r) "(% & HK)". rename H into Hr.
   rewrite fmap_app fmap_cons app_comm_cons big_opL_app. iDestruct "HK" as "[HK [Hu _]]".
   assert (∃ l, l = (x :: K.*1)) as [l Hl]; [by eauto|].
@@ -1007,6 +1136,10 @@ Proof.
   have Hij: i ≠ j; [
   by intros ->; cut (Some a = Some b); [inversion 1|rewrite -Hlkp_a -Hlkp_b]|].
   iSpecialize ("Hb" with "[]"); [done|].
+  iDestruct "Hu" as (uv ud) "(#Hrepr_uv & #Hrepr_ud & Hu)".
+  iDestruct "Ha" as (av ad) "(#Hrepr_av & #Hrepr_ad & Ha)".
+  iDestruct "Hb" as (bv bd) "(#Hrepr_bv & #Hrepr_bd & Hb)".
+
   iApply (Ectxi_ewp_bind (AppRCtx _)). done. rewrite -Hl //=.
   iApply (ewp_mono' with "[Hu]"). { by iApply (get_diff_spec with "Hu"). }
   iIntros (v) "[-> Hu]". iModIntro.
@@ -1015,50 +1148,66 @@ Proof.
   iApply ewp_pure_step. apply pure_prim_step_beta. simpl.
   iApply (Ectxi_ewp_bind (AppRCtx _)). done.
   iApply (Ectxi_ewp_bind (AppRCtx _)). done.
-  iApply (Ectxi_ewp_bind (BinOpRCtx _ _)). done.
-  iApply ewp_pure_step. by apply pure_prim_step_binop. iApply ewp_value. simpl.
-  iApply (Ectxi_ewp_bind (BinOpLCtx _ _)). done.
+
+  iApply (Ectxi_ewp_bind (AppRCtx _)). done.
+  iApply ewp_mono'. { by iApply (nmult_spec with "Heval_b Hrepr_ud"). }
+  iIntros (c) "#Hc". iModIntro. simpl.
+  iApply (ewp_bind (ConsCtx (AppLCtx _)
+                   (ConsCtx (AppRCtx _) EmptyCtx))). done.
   iApply (ewp_mono' with "[Ha]"). { by iApply (get_diff_spec with "Ha"). }
   iIntros (y) "[-> Ha]". iModIntro. simpl.
-  iApply ewp_pure_step. by apply pure_prim_step_binop. iApply ewp_value.
+  iApply ewp_mono'. { by iApply (nadd_spec with "Hrepr_ad Hc"). }
+  iIntros (ad') "#Hrepr_ad'". iModIntro.
   iApply (ewp_mono' with "[Ha]"). { by iApply (set_diff_spec with "Ha"). }
-  iIntros (v) "Ha". iModIntro.
+  iIntros (v) "Ha". iModIntro. iClear "Hrepr_ad Hc". clear c ad.
   iApply (Ectxi_ewp_bind (AppLCtx _)). done.
   iApply ewp_pure_step. apply pure_prim_step_rec. iApply ewp_value. simpl.
   iApply ewp_pure_step. apply pure_prim_step_beta. simpl.
   iApply (Ectxi_ewp_bind (AppRCtx _)). done.
-  iApply (Ectxi_ewp_bind (BinOpRCtx _ _)). done.
-  iApply ewp_pure_step. by apply pure_prim_step_binop. iApply ewp_value. simpl.
-  iApply (Ectxi_ewp_bind (BinOpLCtx _ _)). done.
+  iApply (Ectxi_ewp_bind (AppRCtx _)). done.
+  iApply ewp_mono'. { by iApply (nmult_spec with "Heval_a Hrepr_ud"). }
+  iIntros (c) "#Hc". iModIntro. simpl.
+  iApply (ewp_bind (ConsCtx (AppLCtx _)
+                   (ConsCtx (AppRCtx _) EmptyCtx))). done.
   iApply (ewp_mono' with "[Hb]"). { by iApply (get_diff_spec with "Hb"). }
   iIntros (y) "[-> Hb]". iModIntro. simpl.
-  iApply ewp_pure_step. by apply pure_prim_step_binop. iApply ewp_value.
+  iApply ewp_mono'. { by iApply (nadd_spec with "Hrepr_bd Hc"). }
+  iIntros (bd') "#Hrepr_bd'". iModIntro.
   iApply (ewp_mono' with "[Hb]"). { by iApply (set_diff_spec with "Hb"). }
-  clear v. iIntros (v) "Hb". iModIntro.
+  clear v. iIntros (v) "Hb". iModIntro. iClear "Hrepr_bd Hc". clear c v.
   iExists ((u, (Mult, a, b)) :: K'), r.
   iSplit; [iPureIntro; by rewrite cons_middle app_assoc Hr|].
   rewrite (big_sepL_delete' _ _ _ _ Hlkp_a).
   rewrite (big_sepL_delete' _ _ _ _ Hlkp_b).
   have Hau: a ≠ u. { by intros ->. }
   have Hbu: b ≠ u. { by intros ->. }
-  iClear "Hu". rewrite !interp_snoc !decide_False; try done.
-  rewrite !(diff_interp_cons (eval (emap' {[x:=xv]} (interp K a)))
-                             (eval (emap' {[x:=xv]} (interp K b))));
-    try (by apply lookup_env_extension'); try done.
-  rewrite -!env_extension_app'; [|done].
+  iClear "Hu Hrepr_uv Hrepr_ud". rewrite !interp_snoc !decide_False; try done.
   iSplitL "Ha"; [|iSplitL "Hb"; [|rewrite Hl; iApply (big_sepL_mono with "HK")]].
-  { rewrite //= diff_var_eq diff_var_neq //=.
-    rewrite lookup_total_alt lookup_env_extension' //=.
-    rewrite Nat.mul_0_r !Nat.add_0_r !Nat2Z.inj_add Nat2Z.inj_mul. done.
+  { iExists av, ad'. iFrame. iSplit; [done|]. iApply (repr_proper with "Hrepr_ad'").
+    rewrite !(diff_interp_cons (eval (emap' {[x:=xv]} (interp K a)))
+                               (eval (emap' {[x:=xv]} (interp K b))));
+    try (by apply lookup_env_extension'); try done.
+    rewrite -!env_extension_app'; [|done]. simpl.
+    rewrite //= diff_var_eq diff_var_neq //=.
+    rewrite lookup_total_alt lookup_env_extension' //=. ring.
   }
-  { iIntros (_). rewrite //= diff_var_eq diff_var_neq //=.
-    rewrite lookup_total_alt lookup_env_extension' //=.
-    rewrite Nat.mul_1_r !Nat2Z.inj_add Nat2Z.inj_mul. done.
+  { iIntros (_). iExists bv, bd'. iFrame. iSplit; [done|].
+    iApply (repr_proper with "Hrepr_bd'").
+    rewrite !(diff_interp_cons (eval (emap' {[x:=xv]} (interp K a)))
+                               (eval (emap' {[x:=xv]} (interp K b))));
+    try (by apply lookup_env_extension'); try done.
+    rewrite -!env_extension_app'; [|done]. simpl.
+    rewrite //= diff_var_eq diff_var_neq //=.
+    rewrite (_ : ∀ y, rmult 0 y == 0)%dring; [|intros ?; ring].
+    rewrite lookup_total_alt lookup_env_extension' //=. ring.
   }
   { intros k y Hlkp'. simpl. iIntros "Hy". iIntros (Hkj Hki).
-    iSpecialize ("Hy" $! Hkj Hki). have Hneq'': u ≠ y; [
+    iDestruct ("Hy" $! Hkj Hki) as (yv yd) "(Hyv & Hyd & Hy)".
+    iExists yv, yd. iFrame.
+    have Hneq'': u ≠ y; [
     intros ->; by apply Hnot_in, (elem_of_list_lookup_2 _ k)|].
-    rewrite interp_snoc decide_False; [|done].
+    rewrite interp_snoc decide_False; [|done]. iFrame.
+    iApply (repr_proper with "Hyd").
     rewrite (diff_interp_cons (eval (emap' {[x:=xv]} (interp K a)))
                               (eval (emap' {[x:=xv]} (interp K b))));
     try (by apply lookup_env_extension'); try done.
@@ -1067,7 +1216,7 @@ Proof.
     by intros ->; destruct (NoDup_lookup _ _ _ _ HNoDup Hlkp_a Hlkp')].
     rewrite diff_var_neq //=;[|
     by intros ->; destruct (NoDup_lookup _ _ _ _ HNoDup Hlkp_b Hlkp')].
-    rewrite Nat.mul_0_r Nat.mul_0_l Nat.add_0_r. done. 
+    ring.
   }
 Qed.
 
@@ -1075,7 +1224,7 @@ Lemma run_spec γ x xv (client : val) K (e : expr unit) :
   EWP client #() <| AD_prot (represents γ x) |> {{ y,
     ∃ (r : name), ⌜ y = #r ⌝ ∗ represents γ x r e }} -∗
       handler_inv γ x xv K -∗
-        EWP run client {{ _, backpropagation_inv x xv K e }}.
+        EWP run client <| effs |> {{ _, backpropagation_inv x xv K e }}.
 Proof.
   iIntros "Hclient Hhandler".
   iApply ewp_pure_step. apply pure_prim_step_beta. simpl.
@@ -1124,15 +1273,17 @@ Proof.
       iApply ewp_pure_step. apply pure_prim_step_beta. simpl.
       iApply (Ectxi_ewp_bind (AppRCtx _)). done.
       iApply (Ectxi_ewp_bind (AppRCtx _)). done.
-      iApply (Ectxi_ewp_bind (BinOpRCtx _ _)). done.
+      iApply (Ectxi_ewp_bind (AppRCtx _)). done.
       iApply (ewp_mono' with "[Hhandler]").
       { by iApply (get_val_spec with "Hb Hhandler"). }
-      iIntros (y) "[-> Hhandler]". iModIntro. simpl.
-      iApply (Ectxi_ewp_bind (BinOpLCtx _ _)). done.
+      iIntros (e_bv) "[#Heval_b Hhandler]". iModIntro. simpl.
+      iApply (ewp_bind (ConsCtx (AppLCtx _)
+                       (ConsCtx (AppRCtx _) EmptyCtx))). done.
       iApply (ewp_mono' with "[Hhandler]").
       { by iApply (get_val_spec with "Ha Hhandler"). }
-      iIntros (y) "[-> Hhandler]". iModIntro. simpl.
-      iApply ewp_pure_step. by apply pure_prim_step_binop. iApply ewp_value.
+      iIntros (e_av) "[#Heval_a Hhandler]". iModIntro. simpl.
+      iApply ewp_mono'. { by iApply (nadd_spec with "Heval_a Heval_b"). }
+      iIntros (uv) "#Huv". iModIntro. simpl.
       iApply ewp_mono'. { by iApply mk_spec. }
       iIntros (y). iDestruct 1 as (u) "[-> Hu]".
       iDestruct (handler_inv_fresh_name with "Hu Hhandler") as %Hu_not_in.
@@ -1140,8 +1291,8 @@ Proof.
       iApply ewp_pure_step. apply pure_prim_step_rec. iApply ewp_value. simpl.
       iApply ewp_pure_step. apply pure_prim_step_beta. simpl.
       iApply (Ectxi_ewp_bind (AppRCtx _)). done. simpl.
-      iMod (handler_inv_update _ x xv K u Add a b av bv with "[Hu] Hhandler Ha Hb")
-        as "[Hhandler #Hu]"; [by rewrite Hinterp_a Hinterp_b //= Nat2Z.inj_add|].
+      iMod (handler_inv_update _ x xv K u Add a b av bv uv with "[] Hu Hhandler Ha Hb")
+        as "[Hhandler #Hu]"; [by rewrite Hinterp_a Hinterp_b //=|].
 
       (* Continuation. *)
       iModIntro. iApply (ewp_mono' with "[Hhandler Hk]").
@@ -1180,20 +1331,21 @@ Proof.
       iApply (Ectxi_ewp_bind (AppRCtx _)). done.
       iApply (ewp_mono' with "[Hhandler]").
       { by iApply (get_val_spec with "Ha Hhandler"). }
-      iIntros (y) "[-> Hhandler]". iModIntro. simpl.
+      iIntros (e_av) "[#Heval_a Hhandler]". iModIntro. simpl.
       iApply (Ectxi_ewp_bind (AppLCtx _)). done.
       iApply ewp_pure_step. apply pure_prim_step_rec. iApply ewp_value. simpl.
       iApply ewp_pure_step. apply pure_prim_step_beta. simpl.
       iApply (Ectxi_ewp_bind (AppRCtx _)). done.
       iApply (ewp_mono' with "[Hhandler]").
       { by iApply (get_val_spec with "Hb Hhandler"). }
-      iIntros (y) "[-> Hhandler]". iModIntro. simpl.
+      iIntros (e_bv) "[#Heval_b Hhandler]". iModIntro. simpl.
       iApply (Ectxi_ewp_bind (AppLCtx _)). done.
       iApply ewp_pure_step. apply pure_prim_step_rec. iApply ewp_value. simpl.
       iApply ewp_pure_step. apply pure_prim_step_beta. simpl.
       iApply (Ectxi_ewp_bind (AppRCtx _)). done.
       iApply (Ectxi_ewp_bind (AppRCtx _)). done.
-      iApply ewp_pure_step. by apply pure_prim_step_binop. iApply ewp_value.
+      iApply ewp_mono'. { by iApply (nmult_spec with "Heval_a Heval_b"). }
+      iIntros (uv) "#Huv". iModIntro. simpl.
       iApply ewp_mono'. { by iApply mk_spec. }
       iIntros (y). iDestruct 1 as (u) "[-> Hu]". simpl.
       iDestruct (handler_inv_fresh_name with "Hu Hhandler") as %Hu_not_in.
@@ -1201,14 +1353,13 @@ Proof.
       iApply ewp_pure_step. apply pure_prim_step_rec. iApply ewp_value. simpl.
       iApply ewp_pure_step. apply pure_prim_step_beta. simpl.
       iApply (Ectxi_ewp_bind (AppRCtx _)). done. simpl.
-      iMod (handler_inv_update _ x xv K u Mult a b av bv with "[Hu] Hhandler Ha Hb")
-        as "[Hhandler #Hu]"; [by rewrite Hinterp_a Hinterp_b //= Nat2Z.inj_mul|].
+      iMod (handler_inv_update _ x xv K u Mult a b av bv uv with "[] Hu Hhandler Ha Hb")
+        as "[Hhandler #Hu]"; [by rewrite Hinterp_a Hinterp_b //=|].
 
       (* Continuation. *)
       iModIntro. iApply (ewp_mono' with "[Hhandler Hk]").
       { iApply ("Hk" with "Hu"). by iApply ("IH" with "Hhandler"). }
       iClear "IH".
-
 
       iIntros (v) "Hback_inv". iModIntro.
       iApply (Ectxi_ewp_bind (AppLCtx _)). done.
@@ -1216,21 +1367,23 @@ Proof.
       iApply ewp_pure_step. apply pure_prim_step_beta. simpl.
       rewrite -Hinterp_a -Hinterp_b.
       case (decide (a = b)) as [->|Hab];[
-      by iApply (mult_update_spec_1 with "Hback_inv")|
-      by iApply (mult_update_spec_2 with "Hback_inv")].
+      by iApply (mult_update_spec_1 with "Heval_a Heval_b Hback_inv")|
+      by iApply (mult_update_spec_2 with "Heval_a Heval_b Hback_inv")].
     }
   }
 Qed.
 
-Lemma grad_spec (n : nat) (f : val) (e : expr unit) :
+Lemma grad_spec (f : val) (e : expr unit) :
   (∀ (represents : name → expr unit → iProp Σ) (x : name),
     represents x (ELeaf ()) -∗
       EWP f #x <| AD_prot represents |> {{ y,
         ∃ (r : name), ⌜ y = #r ⌝ ∗ represents r e }})
     -∗
-  EWP grad f #n {{ y, ⌜ y = #(diff (λ _, n) e tt) ⌝ }}.
+  (∀ (n : val) (rn : R),
+    repr n rn -∗
+      EWP grad f n <| effs |> {{ y, repr y (diff (λ _, rn) e tt) }}).
 Proof.
-  iIntros "f_spec".
+  iIntros "f_spec". iIntros (n rn) "#Hn".
   iApply (Ectxi_ewp_bind (AppLCtx _)). done.
   iApply ewp_pure_step. apply pure_prim_step_beta. simpl.
   iApply ewp_pure_step. apply pure_prim_step_rec. iApply ewp_value. simpl.
@@ -1245,21 +1398,22 @@ Proof.
   iApply (Ectxi_ewp_bind (AppRCtx _)). done.
   iApply ewp_pure_step. apply pure_prim_step_rec. iApply ewp_value. simpl.
   iApply (ewp_mono' with "[f_spec Hx]").
-  { iApply fupd_ewp. iMod (handler_inv_alloc with "Hx") as (γ) "Hhandler".
+  { iApply fupd_ewp. iMod (handler_inv_alloc with "Hn Hx") as (γ) "Hhandler".
     iModIntro. iApply (run_spec with "[f_spec] Hhandler").
     iApply ewp_pure_step. apply pure_prim_step_beta. simpl.
     by iApply "f_spec".
   }
   { iIntros (?). iDestruct 1 as (K' r) "[% [Hx _]]". rename H into Hr. iModIntro.
+    iDestruct "Hx" as (uv ud) "(Huv & Hud & Hx)".
     iApply (Ectxi_ewp_bind (AppLCtx _)). done.
     iApply ewp_pure_step. apply pure_prim_step_rec. iApply ewp_value. simpl.
     iApply ewp_pure_step. apply pure_prim_step_beta. simpl.
     iApply (ewp_mono' with "[Hx]"). { by iApply (get_diff_spec with "Hx"). }
-    iIntros (y) "[-> _]". iPureIntro. rewrite Hr.
-    unfold env_extension, diff'. simpl.
+    iIntros (y) "[-> _]". iModIntro. iApply (repr_proper with "Hud").
+    rewrite Hr. unfold env_extension, diff'. simpl.
     rewrite (diff_emap unit name (λ _, x) _ e tt); [|by intros ()].
-    do 3 f_equiv. apply diff_ext. simpl. intros () _.
-    by rewrite lookup_total_alt lookup_insert.
+    rewrite -(diff_ext (λ _ : (), rn)); [done|]. intros () _.
+    simpl. by rewrite lookup_total_alt lookup_insert.
   }
 Qed.
 
